Cleaner assembly with ip used for the well-founded relation

typed-assembly/StaticCode.v
@@ -1,10 +1,14 @@
 (** An assembly language with a static code segment. *)
 Require Import Arith.
+Require Import List.
 Require Import Wellfounded.
 Require Import Relation_Operators.
 
+Import ListNotations.
+
 Set Implicit Arguments.
 
+(** A complete version of [nth] for lists given the right pre-condition. *)
 Fixpoint valid_nth A (l : list A) (n : nat) (H : n < length l) : A.
   destruct n as [|n]; destruct l as [| x l];
     try destruct (lt_n_0 _ H).
@@ -16,79 +20,92 @@ Defined.
 
 Module Instr.
   Inductive t (S : Set) (L : S -> Type)
-    (lt : sigT L -> sigT L -> Prop) (Hwf : well_founded lt)
+    (lt : (nat * sigT L) -> (nat * sigT L) -> Prop) (Hwf : well_founded lt)
     (size : nat) : Type :=
-  | op : forall (f : S -> S),
-    (forall s (l : L s), {l' : L (f s) | lt (existT _ _ l') (existT _ _ l) }) -> t Hwf size
-  | jcc : (forall s, option {n : nat & forall (l : L s), n <= size}) ->
-    (forall s (l : L s), {l' : L s | lt (existT _ _ l') (existT _ _ l) }) -> t Hwf size.
+  | op :
+    (forall s, {s' : S & forall (l : L s), {l' : L s' |
+      forall ip, lt (ip, existT _ _ l') (Datatypes.S ip, existT _ _ l) }}) -> t Hwf size
+  | jcc :
+    (forall s, {next_ip : nat & forall (l : L s), (next_ip <= size) * {l' : L s |
+      forall ip, lt (next_ip, existT _ _ l') (ip, existT _ _ l) }}) -> t Hwf size.
 End Instr.
 
 Module Program.
   Definition t (S : Set) (L : S -> Type)
-    (lt : sigT L -> sigT L -> Prop) (Hwf : well_founded lt)
+    (lt : (nat * sigT L) -> (nat * sigT L) -> Prop) (Hwf : well_founded lt)
     (size : nat) : Type :=
     list (Instr.t Hwf size).
   
+  (** The instruction pointer [ip] is decrementing during the evaluation, down to zero. *)
   Definition eval (S : Set) (L : S -> Type)
-    (lt_L : sigT L -> sigT L -> Prop) (Hwf : well_founded lt_L)
+    (lt_L : (nat * sigT L) -> (nat * sigT L) -> Prop) (Hwf : well_founded lt_L)
     (size : nat) (p : t Hwf size) (Hp_valid : size = length p)
-    : forall (input : {s : S & L s}) (ip : nat) (Hip_valid : ip <= size),
+    : forall (input : nat * {s : S & L s}) (Hip_valid : fst input <= size),
       {s : S & L s}.
     refine (well_founded_induction_type Hwf _ _).
-    intros input eval ip Hip_valid.
-    destruct input as [s l].
+    intros input eval Hip_valid.
+    destruct input as (ip, (s, l)).
     destruct ip as [|ip].
       (* [ip] is null, the program is terminated. *)
       exact (existT _ _ l).
       
+      (* [ip] is not null, one instruction is executed. *)
       refine (let i := valid_nth p (n := ip) _ in _).
         rewrite Hp_valid in Hip_valid.
         apply lt_S_n.
         now apply le_lt_n_Sm.
-      destruct i as [f fl | ptr fl].
+      destruct i as [f | f].
         (* The current instruction is an [op]. *)
         refine (
-          let (l', Hl'_lt_l) := fl s l in
-          eval (existT _ _ l') Hl'_lt_l ip _).
+          let (s', fl) := f s in
+          let (l', Hl'_lt_l) := fl l in
+          eval (ip, existT _ _ l') (Hl'_lt_l _) _).
           now apply le_Sn_le.
         
         (* The current instruction is a [jcc]. *)
-        destruct (ptr s) as [(next_ip, Hptr)|].
-          (* The jump is occuring. *)
           exact (
-            let (l', Hl'_lt_l) := fl s l in
-            eval (existT _ _ l') Hl'_lt_l next_ip (Hptr l)).
-          
-          (* The jump is not occuring. *)
-          refine (
-            let (l', Hl'_lt_l) := fl s l in
-            eval (existT _ _ l') Hl'_lt_l ip _).
-          now apply le_Sn_le.
+            let (next_ip, fl) := f s in
+            let (Hnext_ip, l'_Hl'_lt_l) := fl l in
+            let (l', Hl'_lt_l) := l'_Hl'_lt_l in
+            eval (next_ip, existT _ _ l') (Hl'_lt_l _) Hnext_ip).
   Defined.
 End Program.
 
 Module Test1.
   Import Instr.
   
-  Definition S := nat.
-  Definition L := fun n => prod (3 <= n) nat.
+  Definition S := prod nat nat.
   
-  Definition measure (x : {n : S & L n}) : nat :=
+  Definition L : S -> Prop := fun s =>
+    let (n, ip) := s in
+    3 <= n /\ ip <> 0.
+  
+  Definition measure (x : {s : S & L s}) : nat :=
     match x with
-    | existT _ _ (_, counter) => counter
+    | existT _ (_, ip) _ => ip
     end.
   
   Definition lt (x y : sigT L) : Prop :=
-    
+    measure x < measure y.
+  
+  Lemma lt_wf : well_founded lt.
+    apply well_founded_ltof.
+  Qed.
+  
+  Definition size := 2.
+  
+  Definition dec_ip (f : nat -> nat) (s : S) : S :=
+    let (n, ip) := s in
+    (f n, pred ip).
   
   (** A program where the state is a single natural number, and the logical world
       a proof that it is greater or equal to three. *)
-  Definition test1 : Program.t (fun n => 3 <= n).
-    refine (
-      op (fun _ => 12) _ (
-      op (fun n => n + 1) _ (
-      ret _)));
+  Definition test1 : Program.t lt_wf size.
+    refine [
+      op lt_wf size (dec_ip (fun n => n + 1)) _;
+      op lt_wf size (dec_ip (fun _ => 12)) _]; intros s l.
+      
+      eapply exist.
     auto with *.
   Defined.
 End Test1.
